theories/Borda_Rule_Ref.thy
@@ -1,4 +1,4 @@
-theory Borda_Rule_Ref         
+theory Borda_Rule_Ref
   imports "Verified_Voting_Rule_Construction.Borda_Rule"
           "Compositional_Structures/Basic_Modules/Borda_Module_Ref"  
           "Compositional_Structures/Elect_Composition_Ref"              
